test/dpe/EngineCore.c
@@ -30,6 +30,8 @@ typedef struct _engine_record_t {
 
 INCLUDE (
     module U8 = FStar.UInt8
+    module US = FStar.SizeT
+
 
     noeq
     type engine_record_repr = {
@@ -51,6 +53,13 @@ INCLUDE (
 
     let is_engine_record (r:ref engine_record_t) (p:perm) (repr:engine_record_repr) =
         exists* s. engine_record_t_pred r s ** engine_record_perm s p repr
+
+    // let spec_hash a s = EverCrypt.Hash.Incremental.spec_hash a s
+
+
+    // let cdi_functional_correctness (c0:Seq.seq U8.t) (uds_bytes:Seq.seq U8.t) (repr:engine_record_repr) 
+    // : prop 
+    // = Seq.length uds_bytes == US.v UDS_LEN /\\ c0 == spec_hmac dice_hash_alg (spec_hash dice_hash_alg uds_bytes) (spec_hash dice_hash_alg repr.l0_binary)
 
 )
 
@@ -77,11 +86,55 @@ bool ed25519_verify(ISARRAY() uint8_t *pubk, ISARRAY() uint8_t *hdr, size_t hdr_
 { return false; }
 
 
+
+// val hacl_hash (alg:alg_t)
+//               (src_len: hashable_len)
+//               (src:A.larray U8.t (US.v src_len))
+//               (dst:A.larray U8.t (US.v (digest_len alg)))
+//               (#psrc:perm)
+//               (#src_seq #dst_seq:erased (Seq.seq U8.t))
+//   : stt unit
+//     (pts_to dst dst_seq **
+//      pts_to src #psrc src_seq)
+//     (fun _ ->
+//        pts_to src #psrc src_seq **
+//        pts_to dst (spec_hash alg src_seq))
 REQUIRES("dst |-> 'dst_seq")
 REQUIRES("src |-> Frac 'p 'src_seq")
 ENSURES("src |-> Frac 'p 'src_seq")
 ENSURES("exists* dst_seq. dst |-> dst_seq")
 void hacl_hash (uint8_t alg, size_t src_len, ISARRAY(src_len)uint8_t *src, ISARRAY(DICE_DIGEST_LEN)uint8_t *dst)
+{
+    return;
+}
+
+
+// val hacl_hmac (alg:alg_t { alg == Spec.Hash.Definitions.sha2_256 })
+//               (dst:A.larray U8.t (US.v (digest_len alg)))
+//               (key:A.array U8.t)
+//               (key_len: hashable_len { US.v key_len == A.length key })
+//               (msg:A.array U8.t)
+//               (msg_len: hashable_len { US.v msg_len == A.length msg })
+//               (#pkey #pmsg:perm)
+//               (#dst_seq:erased (Seq.seq U8.t))
+//               (#key_seq:erased (Seq.seq U8.t))
+//               (#msg_seq:erased (Seq.seq U8.t))
+//   : stt unit
+//     (pts_to dst dst_seq **
+//      pts_to key #pkey key_seq **
+//      pts_to msg #pmsg msg_seq)
+//     (fun _ ->
+//        pts_to key #pkey key_seq **
+//        pts_to msg #pmsg msg_seq **
+//        pts_to dst (spec_hmac alg key_seq msg_seq))
+
+REQUIRES("dst |-> 'dst_seq")
+REQUIRES("key |-> Frac 'p 'key_seq")
+REQUIRES("msg |-> Frac 'p 'msg_seq")
+ENSURES("key |-> Frac 'p 'key_seq")
+ENSURES("msg |-> Frac 'p 'msg_seq")
+ENSURES("exists* dst_seq. dst |-> dst_seq")
+void hacl_hmac(uint8_t alg, ISARRAY(DICE_DIGEST_LEN)uint8_t *dst, ISARRAY(key_len)uint8_t *key, size_t key_len, ISARRAY(msg_len)uint8_t *msg, size_t msg_len)
 {
     return;
 }
@@ -92,7 +145,7 @@ RETURNS(b:bool)
 ENSURES("a1 |-> Frac 'p1 's1")
 ENSURES("a2 |-> Frac 'p2 's2")
 ENSURES("pure (b <==> Seq.equal 's1 's2)")
-bool compare (size_t len, ISARRAY(len)uint8_t *a1, ISARRAY(len)uint8_t *a2)
+bool compare(size_t len, ISARRAY(len)uint8_t *a1, ISARRAY(len)uint8_t *a2)
 {
     LEMMA(admit());
     return false;
@@ -117,7 +170,7 @@ RETURNS(b:bool)
 //ENSURES(is_engine_record record p repr)
 //ENSURES(exists* s. scratch |-> s) //remove scratch parameter and all its uses once array allocation is supported
 //Vidush: Removed the scratch parameter since we have support for stack allocated array.
-bool authenticate_l0_image (engine_record_t *record/*, ISARRAY(DICE_DIGEST_LEN)uint8_t *scratch*/)
+bool authenticate_l0_image(engine_record_t *record/*, ISARRAY(DICE_DIGEST_LEN)uint8_t *scratch*/)
 {
     LEMMA(unfold is_engine_record);
     LEMMA(engine_record_t_explode (!record));
@@ -139,5 +192,74 @@ bool authenticate_l0_image (engine_record_t *record/*, ISARRAY(DICE_DIGEST_LEN)u
         return false;
     }
 }
+
+
+// fn compute_cdi
+//   (cdi:A.larray U8.t (SZ.v (digest_len dice_hash_alg)))
+//   (uds:A.larray U8.t (US.v uds_len))
+//   ([@@@ Rust_mut_binder] record:engine_record_t)
+//   (#uds_perm #p:perm)
+//   (#uds_bytes:Ghost.erased (Seq.seq U8.t))
+//   requires pts_to uds #uds_perm uds_bytes
+//         ** pts_to cdi 'c0
+//         ** engine_record_perm record p 'repr
+//   returns record:engine_record_t
+//   ensures engine_record_perm record p 'repr
+//        ** pts_to uds #uds_perm uds_bytes
+//        ** (exists* (c1:Seq.seq U8.t). 
+//             pts_to cdi c1 **
+//             pure (cdi_functional_correctness c1 uds_bytes 'repr))
+// {
+//   A.pts_to_len uds;
+//   let mut uds_digest = [| 0uy; dice_digest_len |];
+//   let mut l0_digest = [| 0uy; dice_digest_len |];
+//   hacl_hash dice_hash_alg uds_len uds uds_digest;
+
+//   unfold engine_record_perm record p 'repr;
+
+//   V.to_array_pts_to record.l0_binary;
+//   hacl_hash dice_hash_alg record.l0_binary_size (V.vec_to_array record.l0_binary) l0_digest;
+//   V.to_vec_pts_to record.l0_binary;
+
+//   fold engine_record_perm record p 'repr;
+
+//   hacl_hmac dice_hash_alg cdi 
+//     uds_digest dice_digest_len
+//     l0_digest dice_digest_len;
+  
+//   record
+// }
+
+
+
+ERASED_ARG(#uds_perm:_)
+ERASED_ARG(#p:_)
+ERASED_ARG(#repr:erased _)
+PRESERVES(is_engine_record record p repr)
+ERASED_ARG(#uds_bytes:erased _)
+PRESERVES("Pulse.Lib.Array.pts_to uds #uds_perm uds_bytes") // ** pts_to cdi 'c0 ** engine_record_perm record p 'repr")
+PRESERVES("Pulse.Lib.Array.pts_to cdi 'c0")
+RETURNS(ref engine_record_t)
+// ENSURES("engine_record_perm record p 'repr \
+//        ** pts_to uds #uds_perm uds_bytes \
+//        ** (exists* (c1:Seq.seq U8.t). \
+//             pts_to cdi c1 ** \
+//             pure (cdi_functional_correctness c1 uds_bytes 'repr))")
+
+engine_record_t *compute_cdi(ISARRAY(DICE_DIGEST_LEN)uint8_t *cdi, ISARRAY(UDS_LEN)uint8_t *uds, engine_record_t *record){
+    LEMMA(unfold is_engine_record);
+    LEMMA(engine_record_t_explode (!record));
+    uint8_t uds_digest[DICE_DIGEST_LEN];
+    uint8_t l0_digest[DICE_DIGEST_LEN];
+    hacl_hash(DICE_HASH_ALG, UDS_LEN, uds, uds_digest);
+    hacl_hash(DICE_HASH_ALG, record->l0_binary_size, record->l0_binary, l0_digest);
+    LEMMA(engine_record_t_recover (!record));
+    LEMMA(fold is_engine_record);
+
+    hacl_hmac(DICE_HASH_ALG, cdi, uds_digest, DICE_DIGEST_LEN, l0_digest, DICE_DIGEST_LEN);
+
+    return record;
+}
+
 
 
