test/general/heap_allocated_array.c
@@ -2,26 +2,33 @@
 #include <stdint.h>
 #include "../include/PulseMacros.h"
 
-REQUIRES(pure (SizeT.v length < 100))
+
+struct foo_struct {
+int a; 
+int b;
+};
+
+REQUIRES(pure (UInt64.v length < 100))
 RETURNS(Int32.t)
-unsigned long foo(size_t length){
-  //ISARRAY(10)int *a = (int*) malloc(sizeof(int) * 10);
+int foo(size_t length){
+  ISARRAY(10)int *a = (int*) malloc(sizeof(int) * 10);
   //This should pass since the call allocates int of sizeof(int)
-  //int *b0 = (int*) malloc(sizeof(int));
+  /*ISARRAY(1)*/ int *b0 = (int*) malloc(sizeof(int));
   //int64_t *b3 = (int64_t*) malloc(sizeof(int64_t));
   //This should Fail since the call allocates int of sizeof(int)
   //int *b1 = (int*) malloc(sizeof(int) * 10);
   //This should Fail since the call allocates int of non constant size
   //Mark this with ISARRAY to tell the compiler its an array 
-  //int *b2 = (int*) malloc(sizeof(int) * length);
-  //ISARRAY(length)int *b = (int*) malloc(sizeof(int) * length);
-  //ISARRAY(length)int *c = (int*) malloc(sizeof(int) * length);
+  ISARRAY(length)int *b2 = (int*) malloc(sizeof(int) * (length * 100));
+  ISARRAY(length)int *b = (int*) malloc(sizeof(int) * length);
+  //ISARRAY(length)int *c = (struct foo_struct*) malloc(sizeof(struct foo_struct) * length);
   
-  //free(a);
-  //free(b0);
+  free(a);
+  free(b0);
   //free(b3);
   //free(b1); 
-  //free(b2);
-  //free(b);
+  free(b2);
+  free(b);
+  //free(c);
   return length;
 }
