test/general/pulse_tutorial_array.c
@@ -6,35 +6,36 @@
 
 INCLUDE ( 
   module SZ = Pulse.Lib.C.SizeT
+  module U64 = FStar.UInt64
  )
 
 ERASED_ARG(#s:erased (Seq.seq int32))
-ERASED_ARG(#p:perm  { SZ.as_int i < Seq.length s })
+ERASED_ARG(#p:perm  { U64.v i < Seq.length s })
 REQUIRES(arr |-> Frac p s)
 RETURNS(v:int32)
 ENSURES(arr |-> Frac p s)
-ENSURES(pure (v == Seq.index s (SZ.as_int i) ))
+ENSURES(pure (v == Seq.index s (U64.v i) ))
 int read_i(ISARRAY() int *arr, size_t i)
 {
     return arr[i];
 }
 
-ERASED_ARG(#s:erased (Seq.seq int32) { SZ.as_int i < Seq.length s })
+ERASED_ARG(#s:erased (Seq.seq int32) { U64.v i < Seq.length s })
 REQUIRES(arr |-> s)
-ENSURES(exists* s1. (arr |-> s1) ** pure (s1 == Seq.upd s (SZ.as_int i) v))
+ENSURES(exists* s1. (arr |-> s1) ** pure (s1 == Seq.upd s (U64.v i) v))
 void write_i(ISARRAY() int *arr, size_t i, int v)
 {
     arr[i] = v;
 }
 
 ERASED_ARG(#s1 #s2 : erased (Seq.seq int32))
-ERASED_ARG(#p:perm { Seq.length s1 = Seq.length s2 && Seq.length s2 = SZ.as_int l })
+ERASED_ARG(#p:perm { Seq.length s1 = Seq.length s2 && Seq.length s2 = U64.v l })
 REQUIRES(a1 |-> Frac p s1)
 REQUIRES(a2 |-> Frac p s2)
 RETURNS(res:int32)
 ENSURES(a1 |-> Frac p s1)
 ENSURES(a2 |-> Frac p s2)
-ENSURES(pure (res==1l <==> (SZ.as_int i < SZ.as_int l && Seq.index s1 (SZ.as_int i) = Seq.index s2 (SZ.as_int i))))
+ENSURES(pure (res==1l <==> (U64.v i < U64.v l && Seq.index s1 (U64.v i) = Seq.index s2 (U64.v i))))
 int compare_elements(ISARRAY() int *a1, ISARRAY() int *a2, size_t l, size_t i)
 {
     if (i < l)
@@ -59,7 +60,7 @@ INCLUDE (
 )
 
 ERASED_ARG(#s1 #s2 : erased (Seq.seq int32))
-ERASED_ARG(#p:perm { Seq.length s1 = Seq.length s2 && Seq.length s2 = SZ.as_int l })
+ERASED_ARG(#p:perm { Seq.length s1 = Seq.length s2 && Seq.length s2 = U64.v l })
 REQUIRES(a1 |-> Frac p s1)
 REQUIRES(a2 |-> Frac p s2)
 RETURNS(res:bool)
@@ -72,19 +73,19 @@ bool compare(ISARRAY() int *a1, ISARRAY() int *a2, size_t l)
     LEMMA(with va1. assert (a1 |-> va1));
     LEMMA(with va2. assert (a2 |-> va2));
     while( compare_elements(a1, a2, l, i) == 1 )
-    INVARIANTS("invariant b.\
-        exists* vi vl.\
-            (a1 |-> va1) ** (a2 |-> va2) ** (* tedious *) \
-            (i |-> vi) ** (va1 |-> Frac p s1) ** (va2 |-> Frac p s2) **\
-            (l |-> vl) **\
-            pure (\
-                Seq.length s1 = SZ.as_int vl /\\
-                Seq.length s2 = SZ.as_int vl /\\
-                SZ.as_int vi <= SZ.as_int vl /\\
-                (b == (SZ.as_int vi < SZ.as_int vl && Seq.index s1 (SZ.as_int vi) = Seq.index s2 (SZ.as_int vi))) /\\
-                (forall (i:nat). i < SZ.as_int vi ==> Seq.index s1 i == Seq.index s2 i)            \
-            )"
-    )
+    INVARIANTS(
+"invariant b. \
+exists* vi vl. \
+(a1 |-> va1) ** (a2 |-> va2) ** (* tedious *) \
+(i |-> vi) ** (va1 |-> Frac p s1) ** (va2 |-> Frac p s2) **\
+(l |-> vl) **\
+pure (\
+Seq.length s1 = U64.v vl /\\
+Seq.length s2 = U64.v vl /\\
+U64.v vi <= U64.v vl /\\
+(b == (U64.v vi < U64.v vl && Seq.index s1 (U64.v vi) = Seq.index s2 (U64.v vi))) /\\
+(forall (i:nat). i < U64.v vi ==> Seq.index s1 i == Seq.index s2 i))"
+)
     {
         i = i + 1;
     }
