test/general/test_union.c
@@ -1,0 +1,39 @@
+#include <stdio.h>
+#include <stdint.h>
+#include <stdbool.h>
+#include "../include/PulseMacros.h"
+
+
+union ab {
+         unsigned int a;
+         bool b;
+};
+
+ERASED_ARG(s:_)
+REQUIRES(pure (Case_a? s))
+REQUIRES(ab_pred x s)
+REQUIRES(pure (UInt32.fits (UInt32.v (Case_a?._0 s) + 1)))
+ENSURES(exists* s'. ab_pred x s')
+void incr_a(union ab *x) {
+  LEMMA(ab_explode !x);
+  LEMMA(rewrite each s as Case_a (Case_a?._0 s));
+  x->a = x->a + 1;
+  LEMMA(ab_recover !x #(Case_a _));
+}
+
+struct stru {
+        int8_t tag;
+        union ab payload;
+};
+
+INCLUDE(
+"let stru_ok (u : ref stru) (s : stru_spec) : slprop =\
+stru_pred u s **\
+pure (\
+match s.tag with\
+| 0y -> Case_a? s.payload\
+| 1y -> Case_b? s.payload\
+| _ -> false\
+)"
+)                                          
+
