test/issue-related/issue52_test.c
@@ -2,6 +2,7 @@
 	
 	
 REQUIRES(exists* v. (x |-> v))
+REQUIRES(pure (length x == 5))
 RETURNS(Int32.t)
 ENSURES(exists* v. (x |-> v))
 int fake_arr(ISARRAY(5) int* x) {
