test/issue-related/issue52_test_2.c
@@ -1,5 +1,7 @@
 #include "../include/PulseMacros.h"
 
+
+REQUIRES(pure (length x == 5))
 REQUIRES(exists* v. (x |-> v))
 RETURNS(Int32.t)
 ENSURES(exists* v. (x |-> v))
