test/issue-related/issue53_test.c
@@ -1,0 +1,17 @@
+#include <stdlib.h>
+#include "../include/PulseMacros.h"
+
+
+RETURNS(res : ref Int32.t)
+ENSURES(exists* v. res |-> v)
+int* foo(int x) {
+	LEMMA(admit());
+	return &x; // bogus
+}
+
+EXPECT_FAILURE()
+RETURNS(Int32.t)
+int bar(int x) {
+	free(foo(x));
+	return 42;
+}
