test/issue-related/issue56_test.c
@@ -1,0 +1,8 @@
+#include "../include/PulseMacros.h"
+
+
+void foo() {
+  int x;
+  LEMMA(assert emp);
+  x = 1;
+}
