test/snapshots/Heap_allocated_array.fst
@@ -7,18 +7,89 @@ open Pulse.Lib.C
 
 
 
+noeq
+type foo_struct = {
+a: ref Int32.t;
+b: ref Int32.t;
+}
+
+[@@erasable]
+noeq
+type foo_struct_spec = {
+a : Int32.t;
+b : Int32.t
+
+}
+
+let foo_struct_pred (x:ref foo_struct) (s:foo_struct_spec) : slprop =
+exists* (y: foo_struct). (x |-> y) **
+(y.a |-> s.a) **
+(y.b |-> s.b)
+
+assume val foo_struct_spec_default : foo_struct_spec
+
+assume val foo_struct_default (foo_struct_var_spec:foo_struct_spec) : foo_struct
+
+ghost
+fn foo_struct_pack (foo_struct_var:ref foo_struct) (#foo_struct_var_spec:foo_struct_spec)
+requires foo_struct_var|-> foo_struct_default foo_struct_var_spec
+ensures exists* v. foo_struct_pred foo_struct_var v ** pure (v == foo_struct_var_spec)
+{ admit() }
+
+ghost
+fn foo_struct_unpack (foo_struct_var:ref foo_struct)
+requires exists* v. foo_struct_pred foo_struct_var v 
+ensures exists* u. foo_struct_var |-> u
+{ admit() }
+
+fn foo_struct_alloc ()
+returns x:ref foo_struct
+ensures freeable x
+ensures exists* v. foo_struct_pred x v
+{ admit () }
+
+fn foo_struct_free (x:ref foo_struct)
+requires freeable x
+requires exists* v. foo_struct_pred x v
+{ admit() }
+
+
+ghost fn foo_struct_explode (x:ref foo_struct) (#s:foo_struct_spec)
+requires foo_struct_pred x s
+ensures exists* (v: foo_struct). (x |-> v) ** (v.a |-> s.a) ** 
+(v.b |-> s.b)
+
+{unfold foo_struct_pred}
+
+
+ghost
+fn foo_struct_recover (x:ref foo_struct) (#a0 : Int32.t)
+(#a1 : Int32.t)
+
+requires exists* (y: foo_struct). (x |-> y) ** 
+(y.a |-> a0) **
+(y.b |-> a1)
+ensures exists* w. foo_struct_pred x w ** pure (w == {a = a0;
+b = a1})
+{fold foo_struct_pred x ({a = a0;
+b = a1}) }
+
 fn foo
-(length : SizeT.t)
-requires pure (SizeT.v length < 100)
+(length : UInt64.t)
+requires pure (UInt64.v length < 100)
 returns Int32.t
 {
-let mut length : SizeT.t = length;
-let mut a : (array Int32.t) = alloc_array #Int32.t 40sz;
+let mut length : UInt64.t = length;
+let mut size_expr0 : SizeT.t = (uint64_to_sizet (int32_to_uint64 10l));
+let mut a : (array Int32.t) = alloc_array #Int32.t !size_expr0;
 let mut b0 : (ref Int32.t) = alloc_ref #Int32.t ();
-let mut size_expr0 : SizeT.t = (uint64_to_sizet (UInt64.mul 4UL (sizet_to_uint64 (! length))));
-let mut b : (array Int32.t) = alloc_array #Int32.t !size_expr0;
+let mut size_expr1 : SizeT.t = (uint64_to_sizet ((UInt64.mul (! length) (int32_to_uint64 100l))));
+let mut b2 : (array Int32.t) = alloc_array #Int32.t !size_expr1;
+let mut size_expr2 : SizeT.t = (uint64_to_sizet (! length));
+let mut b : (array Int32.t) = alloc_array #Int32.t !size_expr2;
 (free_array #Int32.t (! a));
 (free_ref (! b0));
+(free_array #Int32.t (! b2));
 (free_array #Int32.t (! b));
-1l;
+(uint64_to_int32 (! length));
 }
