test/snapshots/Issue52_test_2.fst
@@ -9,7 +9,7 @@ open Pulse.Lib.C
 
 fn fake_arr
 (x : array Int32.t)
-requires pure (length x == SizeT.v 5sz)
+requires pure (length x == 5)
 requires exists* v. (x |-> v)
 returns Int32.t
 ensures exists* v. (x |-> v)
