test/snapshots/Issue53_test.fst
@@ -1,0 +1,28 @@
+module Issue53_test
+
+#lang-pulse
+
+open Pulse
+open Pulse.Lib.C
+
+
+
+fn foo
+(x : Int32.t)
+returns res : ref Int32.t
+ensures exists* v. res |-> v
+{
+let mut x : Int32.t = x;
+admit();
+(x);
+}
+
+[@@expect_failure]
+fn bar
+(x : Int32.t)
+returns Int32.t
+{
+let mut x : Int32.t = x;
+(free_ref (foo (! x)));
+42l;
+}
