test/snapshots/Issue54_test.fst
@@ -10,10 +10,10 @@ open Pulse.Lib.C
 fn compare_elt
 (a1 : array Int32.t)
 (a2 : array Int32.t)
-(i : SizeT.t)
-(len : SizeT.t)
-requires pure (length a2 == SizeT.v len)
-requires pure (length a1 == SizeT.v len)
+(i : UInt64.t)
+(len : UInt64.t)
+requires pure (length a1 == UInt64.v len)
+requires pure (length a2 == UInt64.v len)
 requires exists* v. (a1 |-> v)
 requires exists* v. (a2 |-> v)
 returns b:_Bool
@@ -22,13 +22,13 @@ ensures exists* v. (a2 |-> v)
 {
 let mut a1 : (array Int32.t) = a1;
 let mut a2 : (array Int32.t) = a2;
-let mut i : SizeT.t = i;
-let mut len : SizeT.t = len;
-if((int32_to_bool (bool_to_int32 (SizeT.lt (! i) (! len)))))
+let mut i : UInt64.t = i;
+let mut len : UInt64.t = len;
+if((int32_to_bool (bool_to_int32 (UInt64.lt (! i) (! len)))))
 {
 pts_to_len !a1;
 pts_to_len !a2;
-(int32_to_bool ((bool_to_int32 (Int32.eq (op_Array_Access (! a1) (! i)) (op_Array_Access (! a2) (! i))))));
+(int32_to_bool ((bool_to_int32 (Int32.eq (op_Array_Access (! a1) (uint64_to_sizet (! i))) (op_Array_Access (! a2) (uint64_to_sizet (! i)))))));
 }
 else
 {
