test/snapshots/Issue55_test.fst
@@ -11,21 +11,19 @@ open Pulse.Lib.C
 fn compare
 (a1 : array Int32.t)
 (a2 : array Int32.t)
-(l : SizeT.t)
-requires pure (length a2 == SizeT.v l)
-requires pure (length a1 == SizeT.v l)
+(l : UInt64.t)
 {
 let mut a1 : (array Int32.t) = a1;
 let mut a2 : (array Int32.t) = a2;
-let mut l : SizeT.t = l;
-let mut i : SizeT.t = (int32_to_sizet 0l);
-while((int32_to_bool (if (int32_to_bool ((bool_to_int32 (SizeT.lt (! i) (! l)))))
-then (bool_to_int32 (Int32.eq (op_Array_Access (! a1) (! i)) (op_Array_Access (! a2) (! i))))
+let mut l : UInt64.t = l;
+let mut i : UInt64.t = (int32_to_uint64 0l);
+while((int32_to_bool (if (int32_to_bool ((bool_to_int32 (UInt64.lt (! i) (! l)))))
+then (bool_to_int32 (Int32.eq (op_Array_Access (! a1) (uint64_to_sizet (! i))) (op_Array_Access (! a2) (uint64_to_sizet (! i)))))
 else 0l));
 )
 invariant c. emp
 {
-i := (SizeT.add (! i) (int32_to_sizet 1l));
+i := (UInt64.add (! i) (int32_to_uint64 1l));
 };
-(int32_to_bool ((bool_to_int32 (SizeT.eq (! i) (! l)))));
+(int32_to_bool ((bool_to_int32 (UInt64.eq (! i) (! l)))));
 }
