test/snapshots/Pulse_tutorial_array.fst
@@ -7,57 +7,57 @@ open Pulse.Lib.C
 
 
 
-module SZ = Pulse.Lib.C.SizeT
+module SZ = Pulse.Lib.C.SizeT module U64 = FStar.UInt64
 fn read_i
 (arr : array Int32.t)
-(i : SizeT.t)
+(i : UInt64.t)
 (#s:erased (Seq.seq int32))
-(#p:perm { SZ.as_int i < Seq.length s })
+(#p:perm { U64.v i < Seq.length s })
 requires arr |-> Frac p s
 returns v:int32
 ensures arr |-> Frac p s
-ensures pure (v == Seq.index s (SZ.as_int i) )
+ensures pure (v == Seq.index s (U64.v i) )
 {
 let mut arr : (array Int32.t) = arr;
-let mut i : SizeT.t = i;
-(op_Array_Access (! arr) (! i));
+let mut i : UInt64.t = i;
+(op_Array_Access (! arr) (uint64_to_sizet (! i)));
 }
 
 fn write_i
 (arr : array Int32.t)
-(i : SizeT.t)
+(i : UInt64.t)
 (v : Int32.t)
-(#s:erased (Seq.seq int32) { SZ.as_int i < Seq.length s })
+(#s:erased (Seq.seq int32) { U64.v i < Seq.length s })
 requires arr |-> s
-ensures exists* s1. (arr |-> s1) ** pure (s1 == Seq.upd s (SZ.as_int i) v)
+ensures exists* s1. (arr |-> s1) ** pure (s1 == Seq.upd s (U64.v i) v)
 {
 let mut arr : (array Int32.t) = arr;
-let mut i : SizeT.t = i;
+let mut i : UInt64.t = i;
 let mut v : Int32.t = v;
-(! arr).((! i)) <- (! v);
+(! arr).(uint64_to_sizet (! i)) <- (! v);
 }
 
 fn compare_elements
 (a1 : array Int32.t)
 (a2 : array Int32.t)
-(l : SizeT.t)
-(i : SizeT.t)
+(l : UInt64.t)
+(i : UInt64.t)
 (#s1 #s2 : erased (Seq.seq int32))
-(#p:perm { Seq.length s1 = Seq.length s2 && Seq.length s2 = SZ.as_int l })
+(#p:perm { Seq.length s1 = Seq.length s2 && Seq.length s2 = U64.v l })
 requires a1 |-> Frac p s1
 requires a2 |-> Frac p s2
 returns res:int32
 ensures a1 |-> Frac p s1
 ensures a2 |-> Frac p s2
-ensures pure (res==1l <==> (SZ.as_int i < SZ.as_int l && Seq.index s1 (SZ.as_int i) = Seq.index s2 (SZ.as_int i)))
+ensures pure (res==1l <==> (U64.v i < U64.v l && Seq.index s1 (U64.v i) = Seq.index s2 (U64.v i)))
 {
 let mut a1 : (array Int32.t) = a1;
 let mut a2 : (array Int32.t) = a2;
-let mut l : SizeT.t = l;
-let mut i : SizeT.t = i;
-if((int32_to_bool (bool_to_int32 (SizeT.lt (! i) (! l)))))
+let mut l : UInt64.t = l;
+let mut i : UInt64.t = i;
+if((int32_to_bool (bool_to_int32 (UInt64.lt (! i) (! l)))))
 {
-if((int32_to_bool (bool_to_int32 (Int32.eq (op_Array_Access (! a1) (! i)) (op_Array_Access (! a2) (! i))))))
+if((int32_to_bool (bool_to_int32 (Int32.eq (op_Array_Access (! a1) (uint64_to_sizet (! i))) (op_Array_Access (! a2) (uint64_to_sizet (! i)))))))
 {
 1l;
 }
@@ -76,9 +76,9 @@ module SizeT = Pulse.Lib.C.SizeT
 fn compare
 (a1 : array Int32.t)
 (a2 : array Int32.t)
-(l : SizeT.t)
+(l : UInt64.t)
 (#s1 #s2 : erased (Seq.seq int32))
-(#p:perm { Seq.length s1 = Seq.length s2 && Seq.length s2 = SZ.as_int l })
+(#p:perm { Seq.length s1 = Seq.length s2 && Seq.length s2 = U64.v l })
 requires a1 |-> Frac p s1
 requires a2 |-> Frac p s2
 returns res:_Bool
@@ -88,15 +88,15 @@ ensures pure (res <==> Seq.equal s1 s2)
 {
 let mut a1 : (array Int32.t) = a1;
 let mut a2 : (array Int32.t) = a2;
-let mut l : SizeT.t = l;
-let mut i : SizeT.t = (int32_to_sizet 0l);
+let mut l : UInt64.t = l;
+let mut i : UInt64.t = (int32_to_uint64 0l);
 with va1. assert (a1 |-> va1);
 with va2. assert (a2 |-> va2);
 while((int32_to_bool (bool_to_int32 (Int32.eq (compare_elements (! a1) (! a2) (! l) (! i)) 1l)));
 )
-invariant b.        exists* vi vl.            (a1 |-> va1) ** (a2 |-> va2) ** (* tedious *)             (i |-> vi) ** (va1 |-> Frac p s1) ** (va2 |-> Frac p s2) **            (l |-> vl) **            pure (                Seq.length s1 = SZ.as_int vl /\                Seq.length s2 = SZ.as_int vl /\                SZ.as_int vi <= SZ.as_int vl /\                (b == (SZ.as_int vi < SZ.as_int vl && Seq.index s1 (SZ.as_int vi) = Seq.index s2 (SZ.as_int vi))) /\                (forall (i:nat). i < SZ.as_int vi ==> Seq.index s1 i == Seq.index s2 i)                        )
+invariant b. exists* vi vl. (a1 |-> va1) ** (a2 |-> va2) ** (* tedious *) (i |-> vi) ** (va1 |-> Frac p s1) ** (va2 |-> Frac p s2) **(l |-> vl) **pure (Seq.length s1 = U64.v vl /\Seq.length s2 = U64.v vl /\U64.v vi <= U64.v vl /\(b == (U64.v vi < U64.v vl && Seq.index s1 (U64.v vi) = Seq.index s2 (U64.v vi))) /\(forall (i:nat). i < U64.v vi ==> Seq.index s1 i == Seq.index s2 i))
 {
-i := (SizeT.add (! i) (int32_to_sizet 1l));
+i := (UInt64.add (! i) (int32_to_uint64 1l));
 };
-(int32_to_bool ((bool_to_int32 (SizeT.eq (! i) (! l)))));
+(int32_to_bool ((bool_to_int32 (UInt64.eq (! i) (! l)))));
 }
