test/snapshots/Reverse_test.fst
@@ -9,26 +9,25 @@ open Pulse.Lib.C
 
 fn reverse
 (arr : array UInt32.t)
-(len : SizeT.t)
-requires pure (length arr == SizeT.v len)
+(len : UInt64.t)
 requires exists* s.arr |-> s
-requires pure (length arr == SizeT.v len)
+requires pure (length arr == UInt64.v len)
 ensures exists* s.arr |-> s
 {
 let mut arr : (array UInt32.t) = arr;
-let mut len : SizeT.t = len;
-let mut i : SizeT.t = (int32_to_sizet 0l);
+let mut len : UInt64.t = len;
+let mut i : UInt64.t = (int32_to_uint64 0l);
 with varr. assert arr |-> varr;
 with vlen. assert len |-> vlen;
-while((int32_to_bool (bool_to_int32 (SizeT.lt (! i) (SizeT.div (! len) (int32_to_sizet 2l)))));
+while((int32_to_bool (bool_to_int32 (UInt64.lt (! i) (UInt64.div (! len) (int32_to_uint64 2l)))));
 )
-invariant c. (arr |-> varr) ** (len |-> vlen) ** ( exists* vi. (i |->vi) ** (exists* s. varr |->s) ** pure (c == (vi `SizeT.lt` SizeT.div vlen 2sz)) )
+invariant c. (arr |-> varr) ** (len |-> vlen) ** ( exists* vi. (i |->vi) ** (exists* s. varr |->s) ** pure (c == (vi `UInt64.lt` UInt64.div vlen 2UL)) )
 {
-let mut j : SizeT.t = (SizeT.sub (SizeT.sub (! len) (int32_to_sizet 1l)) (! i));
+let mut j : UInt64.t = (UInt64.sub (UInt64.sub (! len) (int32_to_uint64 1l)) (! i));
 pts_to_len varr;
-let mut tmp : UInt32.t = (op_Array_Access (! arr) (! i));
-(! arr).((! i)) <- (op_Array_Access (! arr) (! j));
-(! arr).((! j)) <- (! tmp);
-i := (SizeT.add (! i) (int32_to_sizet 1l));
+let mut tmp : UInt32.t = (op_Array_Access (! arr) (uint64_to_sizet (! i)));
+(! arr).(uint64_to_sizet (! i)) <- (op_Array_Access (! arr) (uint64_to_sizet (! j)));
+(! arr).(uint64_to_sizet (! j)) <- (! tmp);
+i := (UInt64.add (! i) (int32_to_uint64 1l));
 };
 }
