test/snapshots/Simple_compare_sizet.fst
@@ -1,0 +1,76 @@
+module Simple_compare_sizet
+
+#lang-pulse
+
+open Pulse
+open Pulse.Lib.C
+
+
+
+fn foo
+(i : UInt64.t)
+(j : UInt64.t)
+returns _Bool
+{
+let mut i : UInt64.t = i;
+let mut j : UInt64.t = j;
+if((int32_to_bool (bool_to_int32 (UInt64.lt (! i) (! j)))))
+{
+(int32_to_bool 1l);
+}
+else
+{
+(int32_to_bool 0l);
+};
+}
+
+fn bar
+(i : UInt64.t)
+(j : UInt64.t)
+returns _Bool
+{
+let mut i : UInt64.t = i;
+let mut j : UInt64.t = j;
+if((int32_to_bool (bool_to_int32 (UInt64.lt (! i) (! j)))))
+{
+(int32_to_bool 1l);
+}
+else
+{
+(int32_to_bool 0l);
+};
+}
+
+fn baz
+(i : UInt32.t)
+(j : UInt64.t)
+returns _Bool
+{
+let mut i : UInt32.t = i;
+let mut j : UInt64.t = j;
+if((int32_to_bool (bool_to_int32 (UInt64.lt (uint32_to_uint64 (! i)) (! j)))))
+{
+(int32_to_bool 1l);
+}
+else
+{
+(int32_to_bool 0l);
+};
+}
+
+fn boo
+(i : UInt64.t)
+(j : UInt32.t)
+returns _Bool
+{
+let mut i : UInt64.t = i;
+let mut j : UInt32.t = j;
+if((int32_to_bool (bool_to_int32 (UInt64.lt (! i) (uint32_to_uint64 (! j))))))
+{
+(int32_to_bool 1l);
+}
+else
+{
+(int32_to_bool 0l);
+};
+}
